$$ H\left[\begin{matrix}0 & 1 & 2\\0 & 2 & 3\end{matrix}\right] = 0 \Leftrightarrow H\left[\begin{matrix}0 & 1 & 4\\0 & 1 & 2\end{matrix}\right] = H\left[\begin{matrix}0 & 1 & 3\\0 & 1 & 3\end{matrix}\right] $$
$$ H\left[\begin{matrix}0 & 1 & 2\\0 & 2 & 4\end{matrix}\right] = 0 \Leftrightarrow H\left[\begin{matrix}0 & 1 & 5\\0 & 1 & 2\end{matrix}\right] = H\left[\begin{matrix}0 & 1 & 4\\0 & 1 & 3\end{matrix}\right] $$
$$ H\left[\begin{matrix}0 & 1 & 2\\0 & 2 & 5\end{matrix}\right] = 0 \Leftrightarrow H\left[\begin{matrix}0 & 1 & 6\\0 & 1 & 2\end{matrix}\right] = H\left[\begin{matrix}0 & 1 & 5\\0 & 1 & 3\end{matrix}\right] $$
$$ H\left[\begin{matrix}0 & 1 & 2\\0 & 3 & 4\end{matrix}\right] = 0 \Leftrightarrow H\left[\begin{matrix}0 & 1 & 5\\0 & 1 & 3\end{matrix}\right] = H\left[\begin{matrix}0 & 1 & 4\\0 & 1 & 4\end{matrix}\right] $$
$$ H\left[\begin{matrix}0 & 1 & 2\\0 & j & i - 1\end{matrix}\right] = 0 \Leftrightarrow H\left[\begin{matrix}0 & 1 & i\\0 & 1 & j\end{matrix}\right] = H\left[\begin{matrix}0 & 1 & i - 1\\0 & 1 & j + 1\end{matrix}\right] $$
